small-universe (and extensional) PCMs

pulse/examples/steel/arraystructs/Steel.C.Ref.fst
@@ -1,84 +1,113 @@
 module Steel.C.Ref
 module P = FStar.PCM
+module U = Steel.C.Universe
 open FStar.FunctionalExtensionality
 
 #push-options "--print_universes"
 
-noeq type ref (a: Type u#1) (#b: Type u#b) (q: pcm b): Type u#(max 1 b) = {
+noeq type ref' (a: Type u#0) (b: Type u#b) : Type u#b = {
   p: pcm a;
+  q: pcm b;
   pl: connection p q;
-  r: Steel.Memory.ref a p;
+  r: Steel.Memory.ref (U.raise_t u#0 u#1 a) (fstar_pcm_of_pcm (U.raise_pcm p));
 }
 
-let mpts_to (#p: pcm 'a) (r: Steel.Memory.ref 'a p) = Steel.PCMReference.pts_to r
+let pcm_of_ref' r = r.q
+
+let mpts_to (#a: Type u#1) (#p: P.pcm a) (r: Steel.Memory.ref a p) ([@@@smt_fallback] v: a) = Steel.PCMReference.pts_to r v
+
+let raise_p
+  (#a: Type u#0)
+  (#b: Type u#b)
+  (r: ref' a b)
+: Tot (pcm (U.raise_t u#0 u#1 a))
+= U.raise_pcm r.p
+
+let lower_conn
+  (#a: Type u#0)
+  (#b: Type u#b)
+  (r: ref' a b)
+: Tot (connection (raise_p r) r.p)
+= connection_of_isomorphism (isomorphism_inverse (U.raise_pcm_isomorphism u#0 u#1 r.p))
+
+let raise_pl
+  (#a: Type u#0)
+  (#b: Type u#b)
+  (r: ref' a b)
+: Tot (connection (raise_p r) r.q)
+= lower_conn r `connection_compose` r.pl
 
 let pts_to r v =
-  r.r `mpts_to` r.pl.conn_small_to_large.morph v
-  
-let ref_focus r l = {p = r.p; pl = connection_compose r.pl l; r = r.r}
+  r.r `mpts_to` (raise_pl r).conn_small_to_large.morph v
+
+let ref_focus r #q l = {p = r.p; pl = connection_compose r.pl l; r = r.r; q = q}
 
 let ref_focus_id r = connection_compose_id_right r.pl
 
 let ref_focus_comp r l m
-= connection_eq
-    ((r.pl `connection_compose` l) `connection_compose` m)
-    (r.pl `connection_compose` (l `connection_compose` m))
+= connection_compose_assoc r.pl l m
 
 let focus r l s x =
   let r' = ref_focus r l in
-  A.change_slprop_rel  
+  connection_compose_assoc (lower_conn r) r.pl l;
+  A.change_equal_slprop
     (r `pts_to` s)
-    (r' `pts_to` x)
-    (fun _ _ -> True)
-    (fun m -> ());
+    (r' `pts_to` x);
   A.return r'
 
 let unfocus r r' l x =
-  A.change_slprop_rel  
+  connection_compose_assoc (lower_conn r') r'.pl l;
+  A.change_equal_slprop
     (r `pts_to` x)
     (r' `pts_to` l.conn_small_to_large.morph x)
-    (fun _ _ -> True)
-    (fun m -> ())
 
 let split r xy x y =
+  let c = raise_pl r in
+  let xy2 = Ghost.hide (c.conn_small_to_large.morph xy) in
+  let x2 = Ghost.hide (c.conn_small_to_large.morph x) in
+  let y2 = Ghost.hide (c.conn_small_to_large.morph y) in
+  assert (composable (raise_p r) x2 y2);
   A.change_equal_slprop
     (r `pts_to` xy)
-    (r.r `mpts_to` Ghost.reveal (Ghost.hide (r.pl.conn_small_to_large.morph xy)));
+    (r.r `mpts_to` xy2);
   Steel.PCMReference.split r.r
-    (r.pl.conn_small_to_large.morph xy)
-    (r.pl.conn_small_to_large.morph x)
-    (r.pl.conn_small_to_large.morph y);
+    xy2
+    x2
+    y2;
   A.change_equal_slprop
-    (r.r `mpts_to` Ghost.reveal (Ghost.hide (r.pl.conn_small_to_large.morph x)))
+    (r.r `mpts_to` x2)
     (r `pts_to` x);
   A.change_equal_slprop
-    (r.r `mpts_to` Ghost.reveal (Ghost.hide (r.pl.conn_small_to_large.morph y)))
+    (r.r `mpts_to` y2)
     (r `pts_to` y)
 
 let mgather
-  (#a:Type) (#p:pcm a)
+  (#a:Type) (#p:P.pcm a)
   (r:Steel.Memory.ref a p) (v0:Ghost.erased a) (v1:Ghost.erased a)
-: SteelT (_:unit{composable p v0 v1})
+: SteelT (_:unit{P.composable p v0 v1})
     (mpts_to r v0 `star` mpts_to r v1)
-    (fun _ -> mpts_to r (op p v0 v1))
+    (fun _ -> mpts_to r (P.op p v0 v1))
 = Steel.PCMReference.gather r v0 v1
 
 let gather #a #b #p r x y =
+  let c = raise_pl r in
+  let x2 = Ghost.hide (c.conn_small_to_large.morph x) in
+  let y2 = Ghost.hide (c.conn_small_to_large.morph y) in
   A.change_equal_slprop
     (r `pts_to` x)
-    (r.r `mpts_to` Ghost.reveal (Ghost.hide (r.pl.conn_small_to_large.morph x)));
+    (r.r `mpts_to` x2);
   A.change_equal_slprop
     (r `pts_to` y)
-    (r.r `mpts_to` Ghost.reveal (Ghost.hide (r.pl.conn_small_to_large.morph y)));
+    (r.r `mpts_to` y2);
   mgather r.r
-    (r.pl.conn_small_to_large.morph x)
-    (r.pl.conn_small_to_large.morph y);
+    x2
+    y2;
+  assert (composable (raise_p r) x2 y2);
   assert (
-    let x1 = r.pl.conn_small_to_large.morph x in
-    let y1 = r.pl.conn_small_to_large.morph y in
-    let x2 = r.pl.conn_large_to_small.morph x1 in
-    let y2 = r.pl.conn_large_to_small.morph y1 in
-    Ghost.reveal x == x2 /\ Ghost.reveal y == y2
+    let x' = c.conn_large_to_small.morph x2 in
+    let y' = c.conn_large_to_small.morph y2 in
+    composable p x' y' /\
+    Ghost.reveal x == x' /\ Ghost.reveal y == y'
   );
   A.change_equal_slprop _ (r `pts_to` op p x y)
 
@@ -88,22 +117,20 @@ let ref_read (#p: pcm 'b) (#x: Ghost.erased 'b) (r: ref 'a p)
     (fun _ -> r `pts_to` x)
     (requires fun _ -> True)
     (ensures fun _ x' _ -> compatible p x x')
-= let w = Ghost.hide (r.pl.conn_small_to_large.morph x) in
+= let w = Ghost.hide ((raise_pl r).conn_small_to_large.morph x) in
   A.change_equal_slprop (r `pts_to` x) (r.r `mpts_to` w);
   let w' = Steel.PCMReference.read r.r w in
   A.change_equal_slprop (r.r `mpts_to` w) (r `pts_to` x);
-  let x' = r.pl.conn_large_to_small.morph w' in
-  assert (forall frame . (composable r.p w frame /\ op r.p frame w == w') ==> (
-    let sw = r.pl.conn_large_to_small.morph w in
-    let sw' = r.pl.conn_large_to_small.morph w' in
-    let sframe = r.pl.conn_large_to_small.morph frame in
-    (composable p sw sframe /\ op p sframe sw == sw')
-  ));
+  let x' = (raise_pl r).conn_large_to_small.morph w' in
+  compatible_morphism (raise_pl r).conn_large_to_small w w';
   A.return x'
 
 let ref_upd_act (r: ref 'a 'p) (x: Ghost.erased 'b { ~ (Ghost.reveal x == one 'p) }) (y: Ghost.erased 'b) (f: frame_preserving_upd 'p x y)
 : Tot (M.action_except unit Set.empty (hp_of (r `pts_to` x)) (fun _ -> hp_of (r `pts_to` y)))
-= M.upd_gen Set.empty r.r  (Ghost.hide (r.pl.conn_small_to_large.morph x)) (Ghost.hide (r.pl.conn_small_to_large.morph y)) (r.pl.conn_lift_frame_preserving_upd (|x, y, restricted_frame_preserving_upd_intro f|))
+= let c = raise_pl r in
+  let x' = Ghost.hide (c.conn_small_to_large.morph x) in
+  let y' = Ghost.hide (c.conn_small_to_large.morph y) in
+  M.upd_gen Set.empty r.r x' y' (fstar_fpu_of_fpu (raise_p r) x' y' (c.conn_lift_frame_preserving_upd (|x, y, restricted_frame_preserving_upd_intro f|) ))
 
 let as_action (#p:vprop)
               (#q:vprop)
@@ -118,12 +145,11 @@ let ref_upd r x y f = as_action (ref_upd_act r x y f)
 
 let base_fpu p x y =
   fun _ ->
-  Classical.forall_intro (is_unit p);
   compatible_refl p y;
   y
 
 let pts_to_view_explicit_witinv
-  (#a: Type u#1) (#b: Type u#b) (#p: pcm b)
+  (#a: Type u#0) (#b: Type u#b) (#p: pcm b)
   (r: ref a p)
   (#c: Type u#c)
   (vw: sel_view p c)
@@ -134,22 +160,23 @@ let pts_to_view_explicit_witinv
     (requires (M.interp (pts_to_view_explicit r vw x) m /\ M.interp (pts_to_view_explicit r vw y) m))
     (ensures  (x == y))
   =
+    let c = raise_pl r in
     let x_ = vw.to_carrier x in
     let y_ = vw.to_carrier y in
-    let x' = r.pl.conn_small_to_large.morph x_ in
-    let y' = r.pl.conn_small_to_large.morph y_ in
+    let x' = c.conn_small_to_large.morph x_ in
+    let y' = c.conn_small_to_large.morph y_ in
     M.pts_to_join r.r x' y' m;
-    let z' = FStar.IndefiniteDescription.indefinite_description_ghost a (fun z' -> compatible r.p x' z' /\ compatible r.p y' z') in
-    let frame_x' = FStar.IndefiniteDescription.indefinite_description_ghost a (fun frame_x' -> composable r.p x' frame_x' /\ op r.p frame_x' x' == z') in
-    let frame_y' = FStar.IndefiniteDescription.indefinite_description_ghost a (fun frame_y' -> composable r.p y' frame_y' /\ op r.p frame_y' y' == z') in
-    let frame_x_ = r.pl.conn_large_to_small.morph frame_x' in
-    let frame_y_ = r.pl.conn_large_to_small.morph frame_y' in
-    r.p.comm x' frame_x';
-    r.pl.conn_large_to_small.morph_compose x' frame_x';
-    vw.to_view_frame x (r.pl.conn_large_to_small.morph frame_x');
-    r.p.comm y' frame_y';
-    r.pl.conn_large_to_small.morph_compose y' frame_y';
-    vw.to_view_frame y (r.pl.conn_large_to_small.morph frame_y');
+    let z' = FStar.IndefiniteDescription.indefinite_description_ghost _ (fun z' -> compatible (raise_p r) x' z' /\ compatible (raise_p r) y' z') in
+    let frame_x' = FStar.IndefiniteDescription.indefinite_description_ghost _ (fun frame_x' -> composable (raise_p r) x' frame_x' /\ op (raise_p r) frame_x' x' == z') in
+    let frame_y' = FStar.IndefiniteDescription.indefinite_description_ghost _ (fun frame_y' -> composable (raise_p r) y' frame_y' /\ op (raise_p r) frame_y' y' == z') in
+    let frame_x_ = c.conn_large_to_small.morph frame_x' in
+    let frame_y_ = c.conn_large_to_small.morph frame_y' in
+    op_comm (raise_p r) x' frame_x';
+    c.conn_large_to_small.morph_compose x' frame_x';
+    vw.to_view_frame x (c.conn_large_to_small.morph frame_x');
+    op_comm (raise_p r) y' frame_y';
+    c.conn_large_to_small.morph_compose y' frame_y';
+    vw.to_view_frame y (c.conn_large_to_small.morph frame_y');
     ()
   in
   Classical.forall_intro_3 (fun x y -> Classical.move_requires (aux x y))
